Some work done

src/main.v
@@ -1,3 +1,13 @@
+Require Import Omega.
+Require Import Lia.
+Require Import ssreflect.
+Require Import ssrfun.
+Require Import Coq.ssr.ssrbool.
+
+Notation "a :: b" := (cons a b).
+Notation "[]" := (nil).
+
+
 (* Question 1 *)
 
 Inductive DeBruijn :=
@@ -9,47 +19,281 @@ Check Application (Lambda (Var 0)) (Lambda (Var 0)).
 
 (* Question 2 *)
 
-Fixpoint max_var (t: DeBruijn) (c: nat) : nat :=
+Fixpoint max_var_smaller_n_depth (t: DeBruijn) (n: nat) (depth: nat) : Prop :=
     match t with
-    | Var n => n - c
-    | Lambda tp => max_var tp (c + 1)
-    | Application tp0 tp1 => max (max_var tp0 c) (max_var tp1 c)
+    | Var v => v < n + depth
+    | Lambda tp => max_var_smaller_n_depth tp n (depth + 1)
+    | Application tp0 tp1 => (max_var_smaller_n_depth tp0 n depth) /\ (max_var_smaller_n_depth tp1 n depth)
     end.
 
-Definition var_less_equal_n (T: DeBruijn) (n: nat) :=
-    (max_var T 0) <= n.
+Definition max_var_smaller_n (t: DeBruijn) (n: nat) : Prop := 
+    max_var_smaller_n_depth t n 0.
 
-Definition terme_clos (T: DeBruijn) :=
-    var_less_equal_n T 0.
-
-(* mini is the minimal index of a free variable, that can be substituted *)
-Fixpoint substitution_aux (T: DeBruijn) (index: nat) (mini: nat) (S: DeBruijn) :=
-    match T with
-    | Var n =>
-        match (Nat.eqb index n) with 
-        | true => 
-            match (Nat.leb mini index) with 
-            | true => S
-            | false => Var n
-            end
-        | false => Var n
-        end
-    | Lambda tp => Lambda (substitution_aux tp index (mini + 1) S)
-    | Application tp0 tp1 => Application (substitution_aux tp0 index mini S) (substitution_aux tp1 index mini S)
-    end.
-
-Definition substitution (T: DeBruijn) (index: nat) (S: DeBruijn) :=
-    substitution_aux T index 0 S.
-
-Theorem substitution_clos: forall T: DeBruijn, 
-    terme_clos T -> forall index: nat, forall S: DeBruijn, 
-    (substitution T index S) = T.
+Lemma heredite_0: forall (t: DeBruijn), forall (n: nat), forall (d: nat),
+    (max_var_smaller_n_depth t n d) -> (max_var_smaller_n_depth t (n+1) d).
 Proof.
-    intros.
-    induction T.
+    move => t.
+    induction t.
+    simpl. lia.
+    simpl. intro n. intro d.
+    apply IHt.
+    intro n. intro d.
+    simpl.
+    case. intro H1. intro H2.
+    split.
+    apply IHt1. apply H1.
+    apply IHt2. apply H2.
+Qed.
+    
+Notation "C[ n ]( t )" := (max_var_smaller_n t n).
+
+Lemma inutile_0 : forall (n: nat),
+    n + 0 = n.
+Proof.
+    intro.
+    lia.
 Qed.
 
-Lemma recurrence_var_less: forall T: DeBruijn, forall n: nat,
-    var_less_equal_n T n -> var_less_equal_n T (n + 1).
+Lemma inutile_1 : forall (n: nat),
+    S n = n + 1.
+Proof.
+    intro.
+    lia.
+Qed.
 
+Lemma inutile_2 : forall (n: nat), forall (m: nat), forall (p: nat),
+    n + m + p = n + (m + p).
+Proof.
+    intros.
+    lia.
+Qed.
+
+Lemma heredite_1 : forall (t: DeBruijn), forall (n: nat),
+    C[n](t) -> C[n + 1](t).
+Proof.
+    intros. apply heredite_0. exact H.
+Qed.
+
+Lemma heredite_2 : forall (t: DeBruijn), forall (n: nat), forall (m: nat),
+    C[n](t) -> C[n + m](t).
+Proof.
+    intros.
+    induction m.
+    simpl. rewrite -> inutile_0. exact H.
+    rewrite inutile_1. rewrite <- inutile_2.
+    apply heredite_1 with (t := t) (n := n + m). exact IHm.
+Qed. 
+
+Lemma heredite_3 : forall (t: DeBruijn), forall (n: nat), forall (m: nat),
+    n < m -> C[n](t) -> C[m](t).
+Proof.
+    intros.
+    assert (n + (m - n) = m). lia.
+    rewrite <- H1.
+    apply heredite_2.
+    exact H0.
+Qed.
+
+Definition closed (T: DeBruijn) :=
+    C[0](T).
+
+Notation "C( t )" := (closed t).
+
+Theorem closed_universal : forall (t: DeBruijn),
+    C(t) -> forall (n: nat), C[n](t).
+Proof.
+    intros.
+    induction n.
+    exact H.
+    assert (n+1 = S n).
+    lia.
+    rewrite <- H0.
+    apply heredite_1 with (t := t) (n := n).
+    exact IHn.
+Qed.
+
+
+(* Question 3 *)
+
+Fixpoint correct_free_variable_depth (t: DeBruijn) (depth: nat) :=
+    match t with
+    | Var n => if depth <=? n then Var (n + 1) else Var n
+    | Lambda tp => Lambda (correct_free_variable_depth tp (depth + 1))
+    | Application tp0 tp1 => Application (correct_free_variable_depth tp0 depth) (correct_free_variable_depth tp1 depth)
+    end
+.
+
+Definition correct_free_variable (t: DeBruijn) :=
+    correct_free_variable_depth t 0
+.
+
+Fixpoint substitution (t: DeBruijn) (index: nat) (u: DeBruijn) : DeBruijn :=
+    match t with
+    | Var n => if n =? index then u else (Var n)
+    | Lambda tp => Lambda (substitution tp (index + 1) (correct_free_variable u))
+    | Application tp0 tp1 => Application (substitution tp0 index u) (substitution tp1 index u)
+    end
+.
+
+Notation "t [ y <- u ]" := (substitution t y u) (at level 0).
+
+Lemma aux_0 : forall (n: nat), forall (n0: nat),
+    C[n](Var n0) -> n > n0.
+Proof.
+    intros.
+    induction n.
+    unfold max_var_smaller_n in H.
+    unfold max_var_smaller_n_depth in H.
+    simpl in H. exact H.
+    unfold max_var_smaller_n in H.
+    unfold max_var_smaller_n_depth in H.
+    unfold max_var_smaller_n in IHn.
+    unfold max_var_smaller_n_depth in IHn.
+    simpl in H. lia.
+Qed.
+
+
+(* Thanks a lot to Samuel Vivien! *)
+Lemma aux_0_0 : forall (n: nat), forall (n0: nat),
+    n > n0 -> (Nat.eqb n0 n) = false.
+Proof.
+    intros.
+    destruct (PeanoNat.Nat.eqb_neq n0 n).
+    apply H1.
+    lia.
+Qed.
+
+Lemma aux_0_1 : forall (n: nat), forall (n0: nat), forall (u: DeBruijn),
+    C[n](Var n0) -> (if n0 =? n then u else Var n0) = Var n0.
+Proof.
+    intros.
+    rewrite aux_0_0. apply aux_0. exact H.
+    reflexivity.
+Qed.
+
+Lemma aux_1_0 : forall (t: DeBruijn), forall (u: DeBruijn),
+    u = t -> Lambda u = Lambda t.
+Proof.
+    intros.
+    induction t.
+    rewrite H. reflexivity. 
+    rewrite <- H. reflexivity.
+    rewrite <- H. reflexivity.
+Qed.
+
+Lemma aux_2_0 : forall (t: DeBruijn), forall (n: nat), forall (d: nat),
+    max_var_smaller_n_depth t n (d + 1) -> max_var_smaller_n_depth t (n + 1) d.
+Proof.
+    intro. intro.
+    induction t.
+    simpl.
+    lia.
+    simpl.
+    intro.
+    apply IHt with (d := d + 1).
+    simpl. case. case.
+    simpl. split.
+    apply IHt1 with (d := 0). simpl. exact a.
+    apply IHt2 with (d := 0). simpl. exact b.
+    split.
+    destruct H.
+    apply IHt1 with (d := S n0). exact H.
+    destruct H.
+    apply IHt2 with (d := S n0). exact H0.
+Qed.
+
+Lemma aux_2_1 : forall (t: DeBruijn), forall (n: nat), forall (d: nat),
+    max_var_smaller_n_depth (Lambda t) n d -> max_var_smaller_n_depth t (n + 1) d.
+Proof.
+    intros.
+    induction t.
+    simpl. simpl in H.
+    lia.
+    simpl in H.
+    simpl. apply aux_2_0. exact H.
+    simpl. split.
+    destruct H.
+    apply aux_2_0. exact H.
+    destruct H.
+    apply aux_2_0. exact H0.
+Qed.    
+
+Lemma aux_2_2 : forall (t: DeBruijn), forall (n: nat),
+    C[n](Lambda t) -> C[n + 1](t).
+Proof.
+    intros.
+    simpl. apply aux_2_1. exact H.
+Qed.
+
+Lemma aux_3 : forall (t1: DeBruijn), forall (t2: DeBruijn), forall (n: nat),
+    C[n](Application t1 t2) -> C[n](t1) /\ C[n](t2).
+Proof.
+    intros. 
+    split. 
+    unfold max_var_smaller_n. 
+    unfold max_var_smaller_n in H.
+    unfold max_var_smaller_n_depth in H.
+    destruct H.
+    fold max_var_smaller_n_depth in H.
+    exact H.
+    unfold max_var_smaller_n. 
+    unfold max_var_smaller_n in H.
+    unfold max_var_smaller_n_depth in H.
+    destruct H.
+    fold max_var_smaller_n_depth in H.
+    exact H0.
+Qed.
+
+Theorem substitution_aux : forall (t: DeBruijn), forall (n: nat), 
+    C[n](t) -> forall (u: DeBruijn), substitution t n u = t.
+Proof.
+    intro t. 
+    induction t.
+    simpl. intros. apply aux_0_1. exact H.
+    simpl. intros. apply aux_1_0. 
+    apply IHt with (n := n + 1). apply aux_2_2 with (t := t) (n := n). exact H.
+    intros.
+    simpl. apply aux_3 in H. 
+    destruct H.
+    rewrite IHt1. exact H.
+    rewrite IHt2. exact H0.
+    reflexivity.
+Qed.
+
+Theorem substitution_thm : forall (t: DeBruijn),
+    closed t -> forall (u: DeBruijn), forall (n: nat), substitution t n u = t.
+Proof.
+    intros.
+    apply substitution_aux.
+    apply closed_universal.
+    trivial.
+Qed.
+
+(* Question 4 *)
+
+Fixpoint substitution_multiple_aux (t: DeBruijn) (base: nat) (index: nat) (terms: list DeBruijn) :=
+    match terms with
+    | [] => t
+    | h :: q => substitution_multiple_aux (substitution t (base + index) h) base (index + 1) q
+    end
+.
+
+Definition substitution_multiple (t: DeBruijn) (base: nat) (terms: list DeBruijn) :=
+    substitution_multiple_aux t base 0 terms
+.
+
+Notation "t [ y <l- l ]" := (substitution_multiple t y l) (at level 0).
+
+Theorem substitution_multiple_nil : forall (t: DeBruijn), forall (n: nat),
+    t[n <l- []] = t.
+Proof.
+    intros.
+    unfold substitution_multiple.
+    unfold substitution_multiple_aux.
+    reflexivity.
+Qed.
+
+Theorem substitution_multiple_semi_closed : forall (t: DeBruijn), forall (n: nat), 
+    forall (terms: list DeBruijn),
+    C[n](t) -> substitution_multiple t n terms = t.
 
